src3.0/Vellvm/Dominators/dom_list_tree.v
@@ -1,0 +1,70 @@
+Require Import Coqlib.
+Require Import Maps.
+Require Import syntax.
+Require Import infrastructure_props.
+Require Import Metatheory.
+Require Import Program.Tactics.
+Require Import push_iter.
+
+Inductive DTree : Set :=
+| DT_node : positive -> DTrees -> DTree
+with DTrees : Set :=
+| DT_nil : DTrees
+| DT_cons : DTree -> DTrees -> DTrees
+.
+
+Fixpoint list2tree hd tl := 
+match tl with
+| nil => DT_node hd DT_nil
+| hd'::tl' => DT_node hd (DT_cons (list2tree hd' tl') DT_nil)
+end.
+
+Fixpoint dtree_insert dt parent child tl : DTree :=
+match dt with
+| DT_node l0 dts0 =>
+    if positive_eq_dec parent l0
+    then DT_node l0 (dtrees_insert dts0 child tl)
+    else dt
+end
+with dtrees_insert (dts: DTrees) child tl : DTrees :=
+match dts with
+| DT_nil => DT_cons (list2tree child tl) DT_nil
+| DT_cons dt0 dts0 =>
+    let '(DT_node l0 _) := dt0 in
+    if positive_eq_dec l0 child then 
+      match tl with
+      | child'::tl' => DT_cons (dtree_insert dt0 child child' tl') dts0
+      | _ => dts
+      end
+    else DT_cons dt0 (dtrees_insert dts0 child tl)
+end.
+
+Fixpoint compute_sdom_chains_aux (res: positive -> LDoms.t)
+  (bd: list positive) (acc: list (positive * list positive)) 
+  : list (positive * list positive) :=
+match bd with
+| nil => acc
+| l0 :: bd' =>
+    match res l0 with
+    | Some dts0 =>
+        compute_sdom_chains_aux res bd' ((l0, (rev (l0 :: dts0)))::acc)
+    | None => compute_sdom_chains_aux res bd' acc
+    end
+end.
+
+Definition compute_sdom_chains (res: positive -> LDoms.t) rd
+  : list (positive * list positive) :=
+compute_sdom_chains_aux res rd nil.
+
+Definition create_dtree_from_chain dt chain : DTree :=
+match chain with
+| p::((ch::_) as chain') => dtree_insert dt p ch chain'
+| _ => dt
+end.
+
+Definition create_dtree (pe:positive) (rd:list positive) 
+  (res: positive -> LDoms.t) : DTree :=
+let chains := compute_sdom_chains res rd in
+fold_left 
+  (fun acc elt => let '(_, chain):=elt in create_dtree_from_chain acc chain)
+  chains (DT_node pe DT_nil).
